Complete proof of Partial function version of SST-Transducer composition

Compose_SST_Transducer_Partial.thy
@@ -11,11 +11,18 @@ definition remove_var :: "('x, 'b) update" where
   "remove_var x = []"
 
 definition run_SST :: "('q, 'x, 'a, 'b) SST \<Rightarrow> 'a list \<Rightarrow> 'b list option" where
-  "run_SST sst w = (let q = SST.hat1 (delta sst) (initial sst, w)
-                    in let \<xi> = SST.hat2 (delta sst) (eta sst) (initial sst, w)
-                    in case final sst q of
-                      Some u \<Rightarrow> Some (valuate ((remove_var \<bullet> \<xi> \<bullet> (\<lambda>x. u)) (SOME x :: 'x. True))) |
-                      None \<Rightarrow> None)"
+  "run_SST sst w = 
+    (case final sst (SST.hat1 (delta sst) (initial sst, w)) of
+      Some u \<Rightarrow> Some (valuate ((remove_var \<bullet> (SST.hat2 (delta sst) (eta sst) (initial sst, w) \<bullet> (\<lambda>x. u))) u)) |
+      None   \<Rightarrow> None)"
+
+definition run_SST_hom :: "('q, 'x, 'a, 'b) SST \<Rightarrow> 'a list \<Rightarrow> 'b list option" where
+  "run_SST_hom sst w = 
+    (case final sst (SST.hat1 (delta sst) (initial sst, w)) of
+      Some u \<Rightarrow> Some (valuate ((hat_hom remove_var (hat_hom (SST.hat2 (delta sst) (eta sst) (initial sst, w)) u)))) |
+      None   \<Rightarrow> None)"
+
+
 
 definition \<Delta> :: "('q, 'b) trans
               \<Rightarrow> ('q, 'x) trans \<times> ('z, 'x, 'b) update' \<Rightarrow> ('q, 'z) trans"
@@ -30,6 +37,9 @@ definition H :: "('q, 'b) trans \<Rightarrow> ('q, 'b, 'c) out
   lemma delta2f_apply_hat and eta2f_apply_hat in SST.thy *)
 lemma \<Delta>_assoc: "\<Delta> t (f, \<phi> \<bullet> \<psi>) = \<Delta> t (\<Delta> t (f, \<phi>), \<psi>)"
   sorry
+
+lemma H_assoc_hom: "H tr to (f, \<phi> \<bullet> \<psi>) = H tr to (f, \<phi>) \<bullet> H tr to (\<Delta> tr (f, \<phi>), \<psi>)"
+
 
 lemma H_assoc: "H tr to (f, \<phi> \<bullet> \<psi>) = H tr to (f, \<phi>) \<bullet> H tr to (\<Delta> tr (f, \<phi>), \<psi>)"
   sorry
@@ -49,8 +59,8 @@ definition compose_final :: "('q1, 'x1, 'a, 'b) SST \<Rightarrow> ('q2, 'b, 'c) 
   "compose_final sst td = (\<lambda>(q1, f). 
      case final sst q1 of
        Some u \<Rightarrow>
-         if Transducer.final td (\<Delta> (Transducer.delta td) (f, \<lambda>x. u) (Transducer.initial td, q1))
-         then Some (H (Transducer.delta td) (Transducer.eta td) (f, \<lambda>x. u) (Transducer.initial td, q1)) 
+         if Transducer.final td (\<Delta> (Transducer.delta td) (f, \<lambda>x. u) (Transducer.initial td, u))
+         then Some (H (Transducer.delta td) (Transducer.eta td) (f, \<lambda>x. u) (Transducer.initial td, u)) 
          else None |
        None \<Rightarrow> None)"
 
@@ -103,9 +113,11 @@ next
     by (simp add: Cons.IH H_assoc)
 qed
 
-
 lemma initial_delta: "\<Delta> tr (\<lambda>(q, x). q, remove_var) = (\<lambda>(q, x). q)"
   by (simp add: \<Delta>_def remove_var_def)
+
+lemma initial_delta_remove: "\<Delta> tr (\<lambda>(q, x). q, remove_var \<bullet> \<theta>) (q, x) = \<Delta> tr (\<lambda>(q, x). q, \<theta>) (q, x)"
+  by (simp add: \<Delta>_assoc initial_delta)
 
 lemma initial_eta: "H tr to (\<lambda>(q, x). q, remove_var) = remove_var"
   by (auto simp add: H_def remove_var_def)
@@ -175,8 +187,12 @@ next
     by (cases a, auto simp add: all_alphabet_def valuate_distrib valuate_map)
 qed
 
-lemma valuate_delta_hat: "\<Delta> tr (f, remove_var \<bullet> u) (q, x) = hat1 tr (q, valuate ((remove_var \<bullet> u) x))"
+
+lemma valuate_delta_hat: "\<Delta> tr (\<lambda>(q, x). q, remove_var \<bullet> u) (q, x) = hat1 tr (q, valuate ((remove_var \<bullet> u) x))"
   by (simp add: comp_def \<Delta>_def valuate_delta_hat_string alphabet_remove_var)
+
+lemma valuate_delta_hat_remove: "\<Delta> tr (\<lambda>(q, x). q, u) (q, x) = hat1 tr (q, valuate ((remove_var \<bullet> u) x))"
+  by (simp only: sym[OF valuate_delta_hat] initial_delta_remove)
 
 
 lemma valuate_eta_hat_string:
@@ -201,9 +217,8 @@ lemma valuate_eta_hat_2:
   using assms by (simp add: valuate_eta_hat)
 *)
 
-
-declare [[show_types]]
-theorem can_compose_SST_Transducer_total: 
+(* declare [[show_types]] *)
+theorem can_compose_SST_Transducer: 
   fixes sst::" ('q1, 'x, 'a, 'b) SST" and
         td::"('q2, 'b, 'c) transducer"
   shows
@@ -218,51 +233,55 @@ proof -
   let ?f0 = "\<lambda>(q, x). q"
   let ?q' = "SST.hat1 (SST.delta sst) (SST.initial sst, w)"
   let ?xi = "SST.hat2 (SST.delta sst) (SST.eta sst) (SST.initial sst, w)"
-(*
-  have H_inner: "remove_var \<bullet> ?H (?f0, ?xi) \<bullet> ?H (\<Delta> ?tr (?f0, ?xi), SST2.final sst) 
-               = ?H (?f0, remove_var \<bullet> ?xi \<bullet> SST2.final sst)"
-    by (simp add: H_assoc initial_delta initial_eta)
-  have H_swap: "\<And>\<psi> \<phi> q f x g. (\<psi> \<bullet> \<phi> \<bullet> (\<lambda>(q, f). ?H (f, g) (x, q))) (q, f) = (\<psi> \<bullet> \<phi> \<bullet> ?H (f, g)) (x, q)"
-    by (simp add: comp_def)
-*)
+
   show ?thesis
-(*    apply (simp add: compose_SST_Transducer_def run_SST_def run_total_def) *)
-  proof (cases "SST.final sst (SST.hat1 (SST.delta sst) (SST.initial sst, w))")
+  proof (cases "SST.final sst ?q'")
     case None
     then show ?thesis
       apply (simp add: compose_SST_Transducer_def run_SST_def)
       apply (simp add: Transducer.run_def compose_final_def compose_\<delta>_hat)
       done
   next
-    case (Some a)
-      let ?v = "valuate ((remove_var \<bullet> SST.hat2 (SST.delta sst) (SST.eta sst) (SST.initial sst, w) \<bullet> (\<lambda>x::'x. a)) (SOME x. True))"
-      show ?thesis
-        using Some
-        apply (simp only: Transducer.run_def)
-        apply (simp only: Let_def)
-        apply (simp only: run_SST_def[of sst w])
-        apply (simp only: Let_def option.simps)
-      proof -
-        show "run_SST (compose_SST_Transducer sst td) w =
-              (if transducer.final td  (Transducer.hat1 (transducer.delta td) (transducer.initial td, ?v))
-              then Some (Transducer.hat2 (transducer.delta td) (transducer.eta td) (transducer.initial td, ?v)) else None)"       
-        proof (cases "transducer.final td (Transducer.hat1 (transducer.delta td) (transducer.initial td, ?v))")
-          case True
-          show ?thesis
-          using True sorry (* proof (simp) *)
-       next
-         case False
-         then show ?thesis
-           using Some
-         proof (simp add: compose_final_def compose_\<delta>_hat run_SST_def compose_SST_Transducer_def)
-
-      
+    case (Some out_1st_sst)
+    have q2_finalstate: "\<Delta> (transducer.delta td) 
+           (\<Delta> (transducer.delta td) (\<lambda>(q2, x1). q2, ?xi),
+           \<lambda>x. out_1st_sst)
+          (transducer.initial td, out_1st_sst) 
+        = SST.hat1 (transducer.delta td)
+          (transducer.initial td,
+           valuate ((remove_var \<bullet> (?xi \<bullet> (\<lambda>x. out_1st_sst))) out_1st_sst))"
+            by (simp add: sym[OF \<Delta>_assoc] valuate_delta_hat_remove)
+    then show ?thesis
+      proof (cases "Transducer.final td
+        (SST.hat1 (transducer.delta td)
+          (transducer.initial td,
+           valuate
+            ((remove_var \<bullet> (?xi \<bullet> (\<lambda>x. out_1st_sst))) out_1st_sst)))")
+      have poyoshi: "Transducer.hat2 ?tr ?to
+             (transducer.initial td,
+              valuate ((remove_var \<bullet> ?xi \<bullet> (\<lambda>x. out_1st_sst)) out_1st_sst))
+          = valuate (H ?tr ?to (?f0, remove_var \<bullet> ?xi \<bullet> (\<lambda>x. out_1st_sst)) (transducer.initial td, out_1st_sst))"
+          by (simp add: valuate_eta_hat)
+      case True then show ?thesis 
+        apply (simp add: run_SST_def compose_SST_Transducer_def compose_final_def)
+        apply (auto simp add: Transducer.run_def compose_\<delta>_hat compose_\<eta>_hat True Some q2_finalstate)
+        apply (auto simp add: poyoshi)
+        apply (simp add: H_assoc)
+        apply (simp add: initial_delta initial_eta comp_def)
+        done
+      next
+      case False then show ?thesis proof -
+        have H_inner: "remove_var \<bullet> ?H (?f0, ?xi) \<bullet> ?H (\<Delta> ?tr (?f0, ?xi), \<lambda>x. out_1st_sst) 
+             = ?H (?f0, remove_var \<bullet> ?xi \<bullet> (\<lambda>x. out_1st_sst))"
+           by (simp add: H_assoc initial_delta initial_eta)
+        have LHS: "run_SST (compose_SST_Transducer sst td) w = None" 
+          apply (auto simp add: run_SST_def compose_SST_Transducer_def compose_final_def)
+          apply (auto simp add: compose_\<delta>_hat Some q2_finalstate False)
+          done
+        have RHS: "(case run_SST sst w of None \<Rightarrow> None | Some v \<Rightarrow> Transducer.run td v) = None"
+          by (simp add: run_SST_def Transducer.run_def Some False)
+        then show ?thesis by (simp add: LHS RHS)
+      qed
     qed
-
-
-    apply (simp add: compose_final_def compose_\<delta>_hat compose_\<eta>_hat)
-    apply (simp add: H_swap)
-    apply (simp add: H_inner)
-    apply (simp add: valuate_eta_hat remove_var_def)
-    done
+  qed
 qed
